Change to doc comments

solutions/lang.v
@@ -3,7 +3,7 @@ From iris.heap_lang Require Import lang proofmode notation.
 Section heaplang.
 Context `{!heapGS Σ}.
 
-(*
+(**
   Heaplang is a rather simple language defined on top of iris. It's a
   right to left call by value language reminisent of lambda calculus.
   However it is equiped with a heap as well as multithreading.
@@ -11,87 +11,90 @@ Context `{!heapGS Σ}.
   To see the language in action, let's define a small toy program.
 *)
 Definition prog : expr :=
-  let: "x" := ref #1 in (* Allocate the number 1 on the heap *)
-  "x" <- !"x" + #2;; (* Increment x by 2 *)
-  !"x" (* Read the value of x *).
+  (** Allocate the number 1 on the heap *)
+  let: "x" := ref #1 in
+  (** Increment x by 2 *)
+  "x" <- !"x" + #2;;
+  (** Read the value of x *)
+  !"x".
 
-(*
+(**
   This program should evaluate to 3. To prove this we'll use the
-  weakest precondition `WP`. This let's us specify a post condition we
+  weakest precondition [WP]. This let's us specify a post condition we
   expect to hold if and when the program halts.
 *)
 Lemma wp_prog : ⊢ WP prog {{ v, ⌜v = #3⌝ }}.
 Proof.
   rewrite /prog.
-  (*
+  (**
     Heaplang has a set of tactics describing evaluation of the
     language. The initial step of the program is to allocate the
-    reference to 1. To do this we call `wp_alloc` with a name for the
+    reference to 1. To do this we call [wp_alloc] with a name for the
     location and a name for the knowledge that the location stores 1.
   *)
   wp_alloc l as "Hl".
-  (*
-    As pure steps don't require external knowledge `wp_pures` is able
+  (**
+    As pure steps don't require external knowledge [wp_pures] is able
     to evaluate them automatically.
   *)
   wp_pures.
-  (*
-    Next we load the location `l` using the knowledge that it stores 1.
+  (**
+    Next we load the location [l] using the knowledge that it stores 1.
   *)
   wp_load.
-  (* Then we evaluate the addition *)
+  (** Then we evaluate the addition *)
   wp_pures.
-  (*
-    Storing is handled by `wp_store`.
-    Notice that this updates `Hl`. This only works because we are
+  (**
+    Storing is handled by [wp_store].
+    Notice that this updates [Hl]. This only works because we are
     working in a seperation logic.
   *)
   wp_store.
-  (* Finally we use `wp_load` again *)
+  (** Finally we use [wp_load] again *)
   wp_load.
-  (*
+  (**
     Now that the program is concluded, we are left with a fancy update
     modality. You can usually ignore this modality and simply introduce it.
   *)
   iModIntro.
-  (* Now we are left with a trivial proof that 1+2 = 3 *)
+  (** Now we are left with a trivial proof that 1 + 2 = 3 *)
   done.
 Qed.
 
-(*
+(**
   The full list of evaluation tactics can be found at
   https://gitlab.mpi-sws.org/iris/iris/-/blob/master/docs/heap_lang.md
 *)
 
-(*
+(**
   Let's use this knowledge to prove a specification for a larger
   program.
 *)
 Lemma wp_prog_add_2 : ⊢ WP prog + #2 {{v, ⌜v = #5⌝}}.
 Proof.
   iStartProof.
-  (*
-    The first part of this program is to evaluate `prog`. So we can
-    seperate the program into 2 parts. First we evaluate `prog`, then
-    we take the result and add 2 to it. To do this we can use `wp_bind`.
+  (**
+    The first part of this program is to evaluate [prog]. So we can
+    seperate the program into 2 parts. First we evaluate [prog], then
+    we take the result and add 2 to it. To do this we can use [wp_bind].
   *)
   wp_bind prog.
-  (*
+  (**
     Now we have the problem that our post condition doesn't match the
     one we proved. To fix this we can use monitonicity of WP.
   *)
   iApply wp_mono.
   2: { iApply wp_prog. }
   iIntros "%_ ->".
-  (* And now we can evaluate the rest of the program *)
+  (** And now we can evaluate the rest of the program *)
   wp_pures.
-  (* This post condition is again trivial *)
+  (** This post condition is again trivial *)
   done.
 Qed.
 
-(*
+(**
   The previous proof worked, but it is not very ergonomic.
-  To fix this, we'll make `wp_prog` generic on its post condition.
+  To fix this, we'll make [wp_prog] generic on its post condition.
 *)
 Lemma wp_prog_2 (Φ : val → iProp Σ) :
   (∀ v, ⌜v = #3⌝ -∗ Φ v) -∗ WP prog {{v, Φ v}}.
@@ -105,21 +108,21 @@ Proof.
   by iApply "HΦ".
 Qed.
 
-(* Now the other proof becomes much simpler. *)
+(** Now the other proof becomes much simpler. *)
 Lemma wp_prog_add_2_2 : ⊢ WP prog + #2 {{v, ⌜v = #5⌝}}.
 Proof.
   wp_bind prog.
-  (* Now the proof is on the exact for required by `wp_prog_2` *)
+  (** Now the proof is on the exact for required by [wp_prog_2] *)
   iApply wp_prog_2.
-  (* And the proof proceeds as before *)
+  (** And the proof proceeds as before *)
   iIntros "%_ ->".
   by wp_pures.
 Qed.
 
-(*
+(**
   Hoare triples are an extended version of WP that contains a
   precondition. They are defined as
-  `∀ Φ, Pre -∗ (▷ ∀ r0 .. rn, Post -∗ Φ v) -∗ WP e {{v, Φ v}}`.
+  [∀ Φ, Pre -∗ (▷ ∀ r0 .. rn, Post -∗ Φ v) -∗ WP e {{v, Φ v}}].
   This may seem like very long and complicated definition, so let's
   look at it's parts.
 
@@ -131,23 +134,23 @@ Qed.
   step. And finaly we now have a precondition.
 
   The syntax for Hoare triples is as follows:
-  `{{{ Pre }}} e {{{ r0 .. rn, RET v; Post }}}`
-  - `Pre`: the precondiction that is assumed to hold before the
+  [{{{ Pre }}} e {{{ r0 .. rn, RET v; Post }}}]
+  - [Pre]: the precondiction that is assumed to hold before the
     program runs.
-  - `e`: the program to run.
-  - `r0 .. rn`: the parameters used to define the return value.
-  - `v`: an expression specifying the shape of the return value.
-  - `Post`: the postcondition satisfied after the program has halted.
+  - [e]: the program to run.
+  - [r0 .. rn]: the parameters used to define the return value.
+  - [v]: an expression specifying the shape of the return value.
+  - [Post]: the postcondition satisfied after the program has halted.
 *)
 
-(* Let's consider a function that swaps 2 valued *)
+(** Let's consider a function that swaps 2 valued *)
 Definition swap : val :=
   λ: "x" "y",
   let: "v" := !"x" in
   "x" <- !"y";;
   "y" <- "v".
 
-(* To specify this program we use a Hoare triple *)
+(** To specify this program we use a Hoare triple *)
 Lemma wp_swap (l1 l2 : loc) (v1 v2 : val) :
   {{{l1 ↦ v1 ∗ l2 ↦ v2}}}
     swap #l1 #l2
