solutions/fixpoint.v
@@ -4,7 +4,7 @@ From iris.heap_lang Require Import lang proofmode notation.
 Section proofs.
 Context `{!heapGS Σ}.
 
-(*
+(**
   As we have already seen, we can define a predicate for linked lists
   representing a list of specific values.
 *)
@@ -14,7 +14,7 @@ Fixpoint is_list_of (v : val) (xs : list val) : iProp Σ :=
   | x :: xs => ∃ l : loc, ⌜v = SOMEV #l⌝ ∗ ∃ t, l ↦ (x, t) ∗ is_list_of t xs
   end.
 
-(*
+(**
   However, sometimes we don't care about the exact list and instead
   only want to know that each values of the list satisfy a predicate.
   To do this we could define a predicate for when all elements of a
@@ -31,26 +31,26 @@ Fixpoint all (xs : list val) (Φ : val → iProp Σ) : iProp Σ :=
 Definition is_list (v : val) (Φ : val → iProp Σ) : iProp Σ :=
   ∃ xs, is_list_of v xs ∗ all xs Φ.
 
-(*
+(**
   However this definition is rather anoying to work with, as it
   requires explicitly finding the list of values. Alternatively we
   could define the predicate as the solution to a recursive
   definition. This means defining a function:
-  `F : (A → iProp Σ) → (A → iProp Σ)`
-  A solution is then a function `f` satisfying `f = F f`. Solutions to
-  such equations are called fixpoints as `f` doesn't change under `F`.
+  [F : (A → iProp Σ) → (A → iProp Σ)]
+  A solution is then a function [f] satisfying [f = F f]. Solutions to
+  such equations are called fixpoints as [f] doesn't change under [F].
 *)
 Definition is_list_pre (Φ : val → iProp Σ) (f : val → iProp Σ) (v : val) : iProp Σ :=
   ⌜v = NONEV⌝ ∨ ∃ l : loc, ⌜v = SOMEV #l⌝ ∗ ∃ x t, l ↦ (x, t) ∗ Φ x ∗ f t.
 
-(*
+(**
   Recursive definitions can have multiple fixpoints. Of these there
   are two special fixpoints: The least fixpoint and the greatest fixpoint.
   The least fixpoint coresponds to an inductively defined predicate,
   while the greatest coresponds to coinductively defined predicates.
 
-  These solutions exists when F is monotone. This is handled by the
-  typeclass BiMonoPred.
+  These solutions exists when [F] is monotone. This is handled by the
+  typeclass [BiMonoPred].
 *)
 Global Instance is_list_pre_mono Φ : BiMonoPred (is_list_pre Φ).
 Proof.
@@ -64,7 +64,7 @@ Proof.
       iExists x, t.
       iFrame.
       iApply ("HΨ" with "Ht").
-  - (*
+  - (**
       Additionally to monitonicity. We also need to prove that the
       resulting predicate is time preserving. This is trivial in this
       case as values are discrete.
