theories/invariants.v
@@ -2,10 +2,10 @@ From iris.algebra Require Export excl_auth frac_auth.
 From iris.base_logic.lib Require Export invariants.
 From iris.heap_lang Require Import lang proofmode notation par.
 
-(*
-  Let's make a simple multi-threaded program. We can use `Fork e` to
-  create a new thread to run `e`. As such the following program will
-  race to either update `l` or read `l`. Meaning the resulting value
+(**
+  Let's make a simple multi-threaded program. We can use [Fork e] to
+  create a new thread to run [e]. As such the following program will
+  race to either update [l] or read [l]. Meaning the resulting value
   could be either 0 or 1.
 *)
 Definition prog : expr :=
@@ -22,32 +22,32 @@ Proof.
   rewrite /prog.
   wp_alloc l as "Hl".
   wp_pures.
-  (*
+  (**
     Fork does not have its own tactic. Instead we use its
     specification. This specification forces us to split our resources
     between the threads.
   *)
   wp_apply (wp_fork with "[Hl]").
-  (*
-    As such we have to pick a thread to own `l`. But as both threads
-    need to access `l`, we are stuck.
+  (**
+    As such we have to pick a thread to own [l]. But as both threads
+    need to access [l], we are stuck.
   *)
 Abort.
 
-(*
+(**
   To get around this, we will use invariants. Invariants are written
-  `inv N P` where N is a namespace (Think of it as the name of the
-  invariant), and `P` is the proposition we want to make invariant.
+  [inv N P] where N is a namespace (Think of it as the name of the
+  invariant), and [P] is the proposition we want to make invariant.
   As the name suggests, invariants are propositions that will remain
-  true forever. This allows them to be persistent no matter what P is.
+  true forever. This allows them to be persistent no matter what [P] is.
   
   As stated, invariant need a namespace. This allows invariants to be
   used together as long as they are in different namespaces.
 *)
 Let N := nroot .@ "stuff".
 
-(*
-  In this case we want the invariant to incapsulate ownership of `l`
+(**
+  In this case we want the invariant to incapsulate ownership of [l]
   as well as its posible values.
 *)
 Definition prog_inv (l : loc) : iProp Σ :=
@@ -59,11 +59,11 @@ Proof.
   rewrite /prog.
   wp_alloc l as "Hl".
   wp_pures.
-  (*
+  (**
     To create an invariant we use the lemma
-    `inv_alloc : ▷P -∗ |={E}=> inv N P`.
+    [inv_alloc : ▷P -∗ |={E}=> inv N P].
     In order to deal with the udpdate modality, we will use the iMod
-    tactic rather than iPoseProof or iDestruct.
+    tactic rather than [iPoseProof] or [iDestruct].
   *)
   iMod (inv_alloc N _ (prog_inv l) with "[Hl]") as "#I".
   {
@@ -72,20 +72,20 @@ Proof.
     iFrame.
     by iLeft.
   }
-  (*
+  (**
     As the invariant is persistent, we can now share it between the
     threads.
   *)
   wp_apply wp_fork.
-  - (*
-      We can use the `iInv` to access the resources in the invariant.
+  - (**
+      We can use the [iInv] to access the resources in the invariant.
     *)
     iInv "I" as "(%v & Hl & _)".
-    (*
+    (**
       Opening invariants have certain restrictions. It is only
       posible to open invariants over an atomic step, and after this
       step, we must reestablish the invariant.
-      Further more, the `@ ⊤ \ ↑N`, signifies that the `N` namespace
+      Further more, the [@ ⊤ \ ↑N], signifies that the [N] namespace
       has been opened. As such we wont be able to open it twice at the same step.
     *)
     wp_store.
@@ -106,7 +106,7 @@ Qed.
 
 End proofs.
 
-(*
+(**
   Let's look at another program. This program will create a thread to
   increment a counter. While the main thread will read the counter at
   some point. As such, this program should produce some none negative
@@ -126,7 +126,7 @@ Section proofs.
 Context `{!heapGS Σ}.
 Let N := nroot .@ "other stuff".
 
-(*
+(**
   Our invariant wil simply be that the location points to an integer.
 *)
 Definition prog2_inv (l : loc) : iProp Σ :=
@@ -138,30 +138,30 @@ Proof.
   rewrite /prog2.
   wp_alloc l as "Hl".
   wp_pures.
-  (*
+  (**
     Like before, we allocate the invariant.
   *)
   iMod (inv_alloc N _ (prog2_inv l) with "[Hl]") as "#I".
   { iNext. by iExists 0. }
   wp_apply wp_fork.
   - wp_pure.
-    (* We use löb induction to accent the recursive calls *)
+    (** We use löb induction to accent the recursive calls *)
     iLöb as "IH".
     wp_pures.
-    (* If we now try to open the invariant: *)
+    (** If we now try to open the invariant: *)
     iInv "I" as "[%i Hl]".
-    (*
+    (**
       We run into something different to earlier. This new subgoal
-      `Atomic` is a typeclass, stating that the program should only
+      [Atomic] is a typeclass, stating that the program should only
       consist of a single atomic operation. In this case the typeclass
       search fails, because the program infact consists of two
       operations. So it is not atomic.
     *)
     Undo.
-    (*
+    (**
       To get around this, we will use wp_bind to split the program
       into atomic parts.
-      Notice that the %E is necesary to use the notation.
+      Notice that the [%E] is necesary to use the notation.
     *)
     wp_bind (! _)%E.
     iInv "I" as "[%i Hl]".
@@ -170,8 +170,8 @@ Proof.
     iSplitL "Hl".
     { by iExists i. }
     wp_pures.
-    (*
-      As we know need access to `l` again, we have to do the same
+    (**
+      As we know need access to [l] again, we have to do the same
       trick again.
     *)
     wp_bind (_ <- _)%E.
@@ -193,7 +193,7 @@ Qed.
 
 End proofs.
 
-(*
+(**
   This time we'll use the par operator, to do 2 parallel fetch and
   adds. Again we will only prove that r ends up even.
 *)
@@ -208,7 +208,7 @@ Definition parallel_add : expr :=
 Section parallel_add.
 Context `{!heapGS Σ, !spawnG Σ}.
 
-(* The invariant is thus that r points to an even integer. *)
+(** The invariant is thus that r points to an even integer. *)
 Definition parallel_add_inv (r : loc) : iProp Σ :=
   ∃ n : Z, r ↦ #n ∗ ⌜Zeven n⌝.
 
@@ -225,9 +225,9 @@ Proof.
     iExists 0.
     iFrame.
   }
-  (*
+  (**
     We don't need information back from the threads, so we will simply
-    use (λ _, True) as the post conditions.
+    use [λ _, True] as the post conditions.
   *)
   wp_apply (wp_par (λ _, True%I) (λ _, True%I)).
   - iInv "I" as "(%n & Hr & >%Hn)".
