theories/persistently.v
@@ -4,39 +4,39 @@ From iris.proofmode Require Import proofmode.
 Section proofs.
 Context {Σ : gFunctors}.
 
-(*
+(**
   Thus far we've seen the pure context (the coq context) and the
   spatial context. Iris proofmode has a 3rd context, called the
-  inituitionistic context or (for `iProp`) persistent context.
+  inituitionistic context or (for [iProp]) persistent context.
   These are proposisitions that act like propositions in an
   inituitionistic logic. Namely, they are reusable. These propositions
   need not however be pure as they can still depend on resurces. Just
-  like the pure modality, we also have a persistently modality `□ P`.
+  like the pure modality, we also have a persistently modality [□ P].
   It turns arbitrary Iris propositions into a stronger persistent
-  proposition. Persistent proposistions are thus those `P` such that
-  `P ⊢ □ P`. Iris identifies these proposisition using the typeclass
-  `Persistent`. In fact, all pure propositions are persistent.
+  proposition. Persistent proposistions are thus those [P] such that
+  [P ⊢ □ P]. Iris identifies these proposisition using the typeclass
+  [Persistent]. In fact, all pure propositions are persistent.
 *)
 Lemma pers_ex (P Q : iProp Σ) `{!Persistent P} : P -∗ Q -∗ P ∗ Q.
 Proof.
-  (*
+  (**
     We are allowed to put persistent hypotheses into the spacial
     context. This will make the proofmode treat the hypothesis as
     though it wasn't persistent.
   *)
   iIntros "HP HQ".
-  (*
+  (**
     The introduction pattern "#_" allows us to place a hypotheses into
     the persistent context.
   *)
   iDestruct "HP" as "#HP".
   iSplitR.
-  - (*
+  - (**
       Notice that event though I asked Iris to move all hypotheses
       into the second subgoal, I still kept "HP".
     *)
     iApply "HP".
-  - (* And "HP" is also present in this subgoal *)
+  - (** And "HP" is also present in this subgoal *)
     iApply "HQ".
 Qed.
 
@@ -44,15 +44,15 @@ Lemma pers_sep (P : iProp Σ) `{!Persistent P} : P ⊢ P ∗ P.
 Proof.
   (* FILL IN HERE *) Admitted.
 
-(*
-  Persistent propositions satisfy a lot of nice proporties simply by being duplicable (P ⊢ P ∗ P)
-  For example, `P ∧ Q` and `P ∗ Q` coincide, when either `P` or `Q` is persistent.
-  Likewise, `P → Q` and `P -∗ Q` coincide, when `P` is persistent.
+(**
+  Persistent propositions satisfy a lot of nice proporties simply by being duplicable [P ⊢ P ∗ P]
+  For example, [P ∧ Q] and [P ∗ Q] coincide, when either [P] or [Q] is persistent.
+  Likewise, [P → Q] and [P -∗ Q] coincide, when [P] is persistent.
 *)
 Check bi.persistent_and_sep.
 Check bi.impl_wand.
 
-(* Iris proofmode knows these facts, and allows `iSplit` to introduce `∗` when one of its arguements are persistent. *)
+(** Iris proofmode knows these facts, and allows [iSplit] to introduce [∗] when one of its arguements are persistent. *)
 
 
 End proofs.
