theories/pure.v
@@ -4,18 +4,18 @@ From iris.proofmode Require Import proofmode.
 Section proofs.
 Context {Σ : gFunctors}.
 
-(*
-  Turnstyle can be used as a unary operator to ask whether a
+(**
+  Turnstyle can be used as a unary operator to as whether a
   proposition follows from the empty context. Here we locally specify
-  that we want to talk about Iris propositions over Σ.
+  that we want to talk about Iris propositions over [Σ].
   This is useful when stating lemmas that don't depend on generic Iris
   propositions.
 *)
 Local Notation "⊢ P" := (⊢@{iPropI Σ} P).
 
-(*
+(**
   Coq propositions can be embeded into iris using the pure modality
-  `⌜ϕ⌝`. Pure propositions can be introduced using `iPureIntro`. This
+  [⌜ϕ⌝]. Pure propositions can be introduced using [iPureIntro]. This
   will exit Iris proofmode, throwing away the Iris context. Pure
   propositions can be eleminated using the introduction pattern "%_".
 *)
@@ -32,16 +32,16 @@ Proof.
   iApply "HP".
 Qed.
 
-(*
+(**
   Iris has a class of propositions we call pure.
-  These are the propositions `P` that are bientailed by `⌜ϕ⌝` for
-  some Φ. Iris has a 2 typeclasses `IntoPure` and `FromPure` to
+  These are the propositions [P] that are bientailed by [⌜ϕ⌝] for
+  some Φ. Iris has a 2 typeclasses [IntoPure] and [FromPure] to
   identify such propositions.
 *)
 
 Lemma true_intro : ⊢ True.
 Proof.
-  iPureIntro. (*True is pure*)
+  iPureIntro. (* True is pure*)
   constructor.
 Qed.
 
@@ -57,20 +57,20 @@ Proof.
   split; reflexivity.
 Qed.
 
-(*
+(**
   The pure modality allows us to state the most important property.
   Namely soundness. Iris is only a usefull extension because we can
   extract knowledge from Iris out to the Coq metalogic.
 
-  Soundness is proved in the `uPred_primitive.pure_soundness` lemma
-  stating: ∀ φ, (True ⊢ ⌜φ⌝) → φ
+  Soundness is proved in the [uPred_primitive.pure_soundness] lemma
+  stating: [∀ φ, (True ⊢ ⌜φ⌝) → φ]
 
   This means that anything proved inside the Iris logic is as true as
   anything proved in Coq.
 *)
 
-(*
-  ⌜_⌝ turns Coq propositions into Iris propositions, while ⊢_ turns
+(**
+  [⌜_⌝] turns Coq propositions into Iris propositions, while [⊢ _] turns
   Iris propositions into Coq propositions. These operations aren't
   inverses, but they are related.
 *)
